JSON.lean
@@ -1,0 +1,61 @@
+import Soda.Grape
+import Soda.Grape.Text
+import Map
+
+open Grape
+open Function
+
+/--
+The most important part of this was copied from [Ash](https://github.com/meoowers/ash/blob/main/Ash/JSON.lean).
+I haven't used the lib directly because of a mismatch on lake-manifest versions, but
+credits go to Sofia and Gabi.
+-/
+
+inductive JSON where
+  | num : Int → JSON
+  | bool : Bool → JSON
+  | null : JSON
+  | str : String → JSON
+  | arr : List JSON → JSON
+  | obj : Map String JSON → JSON
+  deriving Inhabited, Repr
+
+def JSON.token : Grape α → Grape α := Text.trailing
+
+def JSON.pString : Grape String :=
+  string "\"" *> Text.takeToStr (· != 34) <* string "\""
+
+def JSON.number : Grape Nat :=
+  Text.number
+
+def JSON.space : Grape Unit := list (oneOf " \n\r\t") *> Grape.pure ()
+
+partial def JSON.expr : Grape JSON := token $
+        (str <$> label "string" pString)
+    <|> (num <$> label "number" number)
+    <|> ((λ_ => JSON.null)       <$> label "null" (string "null"))
+    <|> ((λ_ => JSON.bool true)  <$> label "true" (string "true"))
+    <|> ((λ_ => JSON.bool false) <$> label "false" (string "false"))
+    <|> (arr <$> (string "[" *> space *> sepBy expr (space *> (token $ string ",") <* space) <* space <* (token $ string "]")))
+    <|> (obj <$> (string "{" *> space *> sepBy pair (space *> (token $ string ",") <* space) <* space <* (token $ string "}")))
+  where
+    pair := Prod.mk <$> (JSON.pString <* (space *> (token $ string ":") <* space)) <*> expr
+
+instance : Coe String JSON where
+  coe s := JSON.str s
+
+instance : Coe Nat JSON where
+  coe n := JSON.num n
+
+instance : Coe (List JSON) JSON where
+  coe l := JSON.arr l
+
+instance [Coe α JSON] : Coe (Option α) JSON where
+  coe
+    | none => JSON.null
+    | some a => a
+
+def JSON.parse (s: String) : Option JSON :=
+  match Grape.run JSON.expr (s.toSlice) with
+  | Result.done res _ => some res
+  | _                 => none
