Main.lean
@@ -1,6 +1,29 @@
 import Rinha
+import Init.Data.Repr
 
 open Rinha.Environment
 
-def main : IO Unit :=
-  IO.println s!"Hello, {hello}!"
+def parseWithIOError (value : String) : IO JSON := do
+  match JSON.parse value with
+  | Option.some json => pure json
+  | Option.none => throw (IO.userError "Invalid JSON value")
+
+def convertWithIOError (value : JSON) : IO Rinha.Term.Program := do
+  match Rinha.Term.Program.from_JSON value with
+  | Except.ok term => pure term
+  | Except.error error => throw (IO.userError error)
+
+def parseAndConvert (fileName : String) : IO Rinha.Term.Program := do
+  let read ← IO.FS.readFile fileName
+  let json ← parseWithIOError read
+  convertWithIOError json
+
+def printRepr [Repr α] : α → IO Unit := IO.println ∘ repr
+
+def main : IO Unit := do
+  let rinha ← parseAndConvert "rinha.json"
+  printRepr rinha
+  let fib ← parseAndConvert "fib.json"
+  printRepr fib
+  let sum ← parseAndConvert "sum.json"
+  printRepr sum
