Rinha/Term.lean
@@ -1,38 +1,40 @@
+import JSON
+
 namespace Rinha.Term
 
 inductive BinOp
 | Add | Sub | Mul | Div | Rem | Eq | Neq | Lt | Gt | Lte | Gte | And | Or
-deriving Repr
+deriving Repr, BEq, DecidableEq
 
 structure WithLocation (α : Type) where
   value : α
-deriving Repr
+deriving Repr, BEq, DecidableEq
 
 structure Binary (α : Type) where
   lhs : α
   rhs : α
   op : BinOp
-deriving Repr
+deriving Repr, BEq, DecidableEq
 
 def Parameter := WithLocation String
-deriving Repr
+deriving Repr, BEq, DecidableEq
 
 structure Function (α : Type) where
   parameters : List Parameter
   value : α
-deriving Repr
+deriving Repr, BEq, DecidableEq
 
 structure Let (α : Type) where
   name : Parameter
   value : α
   next : α
-deriving Repr
+deriving Repr, BEq, DecidableEq
 
 structure If (α : Type) where
   condition : α
   then' : α
   otherwise : α
-deriving Repr
+deriving Repr, BEq, DecidableEq
 
 inductive Term
 | Int : Int → Term
@@ -48,7 +50,149 @@ inductive Term
 | Second : Term → Term
 | Tuple : Term → Term → Term
 | Var : String → Term
+deriving Repr, BEq
+
+def may_be_bool : Term → Prop
+| Term.Boolean _ => true
+| Term.If {then', otherwise, ..} => may_be_bool then' ∨ may_be_bool otherwise
+| Term.Function {value, ..} => may_be_bool value
+| Term.First (Term.Tuple lhs _) => may_be_bool lhs
+| Term.Second (Term.Tuple _ rhs) => may_be_bool rhs
+| _ => false
+
+def may_be_int : Term → Prop
+| Term.Int _ => true
+| Term.If {then', otherwise, ..} => may_be_bool then' ∨ may_be_bool otherwise
+| Term.Function {value, ..} => may_be_bool value
+| Term.First (Term.Tuple lhs _) => may_be_bool lhs
+| Term.Second (Term.Tuple _ rhs) => may_be_bool rhs
+| _ => false
+
+instance : Coe α (Except String α) where
+  coe x := Except.ok x
+
+def BinOp.from_string : String → Except String BinOp
+| "Add" => BinOp.Add
+| "Sub" => BinOp.Sub
+| "Mul" => BinOp.Mul
+| "Div" => BinOp.Div
+| "Rem" => BinOp.Rem
+| "Eq" => BinOp.Eq
+| "Neq" => BinOp.Neq
+| "Lt" => BinOp.Lt
+| "Gt" => BinOp.Gt
+| "Lte" => BinOp.Lte
+| "Gte" => BinOp.Gte
+| "And" => BinOp.And
+| "Or" => BinOp.Or
+| _ => Except.error "invalid binary operation"
+
+def Parameter.from_JSON : JSON → Except String Parameter
+| JSON.obj fields =>
+  match fields["text"]? with
+  | JSON.str text => pure {value := text}
+  | _ => Except.error "expected a parameter"
+| _ => Except.error "expected a parameter"
+
+partial def Term.from_JSON : JSON → Except String Term
+| JSON.obj fields =>
+  match fields["kind"]? with
+  | "Int" =>
+    match fields["value"]? with
+    | JSON.num n => Term.Int n
+    | _ => Except.error "expected a number"
+  | "Str" =>
+    match fields["value"]? with
+    | JSON.str s => Term.Str s
+    | _ => Except.error "expected a string"
+  | "Boolean" =>
+    match fields["value"]? with
+    | JSON.bool b => Term.Boolean b
+    | _ => Except.error "expected a boolean"
+  | "Tuple" =>
+    match fields["first"]?, fields["second"]? with
+    | Option.some fst, Option.some snd => do
+      let fst ← from_JSON fst
+      let snd ← from_JSON snd
+      Term.Tuple fst snd
+    | _, _ => Except.error "expected a tuple"
+  | "Binary" =>
+    match fields["lhs"]?, fields["rhs"]?, fields["op"]? with
+    | Option.some lhs, Option.some rhs, Option.some (JSON.str op) => do
+      let lhs ← from_JSON lhs
+      let rhs ← from_JSON rhs
+      let op ← BinOp.from_string op
+      Term.Binary {lhs, rhs, op}
+    | _, _, _ => Except.error "expected a binary operation"
+  | "Call" =>
+    match fields["callee"]?, fields["arguments"]? with
+    | Option.some callee, Option.some (JSON.arr args) => do
+      let callee ← from_JSON callee
+      let args ← args.mapM from_JSON
+      Term.Call callee args
+    | _, _ => Except.error "expected a function call"
+  | "Function" =>
+    match fields["parameters"]?, fields["value"]? with
+    | Option.some (JSON.arr params), Option.some value => do
+      let parameters ← params.mapM Parameter.from_JSON
+      let value ← from_JSON value
+      Term.Function {parameters, value}
+    | _, _ => Except.error "expected a function"
+  | "First" =>
+    match fields["value"]? with
+    | Option.some value => do
+      let value ← from_JSON value
+      Term.First value
+    | _ => Except.error "expected a first projection"
+  | "Second" =>
+    match fields["value"]? with
+    | Option.some value => do
+      let value ← from_JSON value
+      Term.Second value
+    | _ => Except.error "expected a second projection"
+  | "Let" =>
+    match fields["name"]?, fields["value"]?, fields["next"]? with
+    | Option.some name, Option.some value, Option.some next => do
+      let name ← Parameter.from_JSON name
+      let value ← from_JSON value
+      let next ← from_JSON next
+      Term.Let {name, value, next}
+    | _, _, _ => Except.error "expected a let binding"
+  | "If" =>
+    match fields["condition"]?, fields["then"]?, fields["otherwise"]? with
+    | Option.some condition, Option.some then', Option.some otherwise => do
+      let condition ← from_JSON condition
+      let then' ← from_JSON then'
+      let otherwise ← from_JSON otherwise
+      Term.If {condition, then', otherwise}
+    | Option.none, _, _ => Except.error "expected a condition"
+    | _, Option.none, _ => Except.error "expected a then branch"
+    | _, _, Option.none => Except.error "expected an otherwise branch"
+  | "Print" =>
+    match fields["value"]? with
+    | Option.some value => do
+      let value ← from_JSON value
+      Term.Print value
+    | _ => Except.error "expected a print expression"
+  | "Var" =>
+    match fields["text"]? with
+    | Option.some (JSON.str name) => Term.Var name
+    | _ => Except.error "expected a variable"
+  | _ => Except.error "invalid Term kind"
+| _ => Except.error "invalid JSON"
+
+structure Program where
+  name : String
+  expression : Term
 deriving Repr
 
+def Program.from_JSON : JSON → Except String Program
+| JSON.obj fields =>
+  match fields["name"]?, fields["expression"]? with
+  | Option.some (JSON.str name), Option.some expression => do
+    let expression ← Term.from_JSON expression
+    pure {name, expression}
+  | _, _ => Except.error "expected a program"
+| _ => Except.error "expected a program"
 
 end Rinha.Term
